Pair_Graph/Pair_Graph_Specs.thy
@@ -12,54 +12,83 @@ text \<open>We develop a locale modelling an abstract data type (ADT) which abst
       We then show that this ADT can be implemented using existing implementations of the \<open>set\<close> ADT.
 \<close>
 
-locale Set_Choose = Set empty insert delete isin t_set invar
-for empty insert delete isin t_set invar +
+locale Set_Choose = Set 
+  where set = t_set for t_set +
 fixes sel ::"'m \<Rightarrow> 'a"
-assumes choose: "t_set m \<noteq> {} \<Longrightarrow> sel m \<in> t_set m"
+assumes choose: "s \<noteq> empty \<Longrightarrow> isin s (sel s)"
+begin
+
+declare set_empty[simp] set_isin[simp] set_insert[simp] set_delete[simp]
+        invar_empty[simp] invar_insert[simp] invar_delete[simp] choose[simp]
+
+subsection \<open>Abstraction lemmas\<close>
+
+text \<open>These are lemmas for automation. Their purpose is to remove any mention of the locale set ADT
+      constructs and replace it with Isabelle's native sets.\<close>
+
+lemma choose'[simp, intro,dest]:
+  "s \<noteq> empty \<Longrightarrow> invar s \<Longrightarrow> sel s \<in> t_set s"
+  by(auto simp flip: set_isin)
+
+lemma choose''[intro]:
+  "invar s \<Longrightarrow> s \<noteq> empty \<Longrightarrow> t_set s \<subseteq> s' \<Longrightarrow> sel s \<in> s'"
+  by(auto simp flip: set_isin)
+
+lemma emptyD[dest]:
+           "s = empty \<Longrightarrow> t_set s = {}"
+           "s \<noteq> empty \<Longrightarrow> invar s \<Longrightarrow> t_set s \<noteq> {}"
+           "empty = s \<Longrightarrow> t_set s = {}"
+           "empty \<noteq> s \<Longrightarrow> invar s \<Longrightarrow> t_set s \<noteq> {}"
+ using local.set_empty
+ by auto
+
+end
+
 
 locale Adj_Map_Specs = 
- adj: Map adj_empty adj_update adj_delete adj_lookup adj_inv +
+ adj: Map 
+ where update = update and invar = adj_inv +
 
- neighb: Set_Choose neighb_empty neighb_insert neighb_delete neighb_isin neighb_set neighb_inv neighb_sel
+ neighb: Set_Choose
+where empty = neighb_empty and delete = neighb_delete and insert = neighb_insert and invar = neighb_inv
+      and isin = isin
 
- for adj_empty :: "'adj" and adj_update :: "'a \<Rightarrow> 'neighb \<Rightarrow> 'adj \<Rightarrow> 'adj" and
-     adj_delete :: "'a \<Rightarrow> 'adj \<Rightarrow> 'adj" and adj_lookup :: "'adj \<Rightarrow> 'a \<Rightarrow> 'neighb option" and
-     adj_inv :: "'adj \<Rightarrow> bool"  and
+ for update :: "'a \<Rightarrow> 'neighb \<Rightarrow> 'adj \<Rightarrow> 'adj" and adj_inv :: "'adj \<Rightarrow> bool"  and
 
-     neighb_empty :: "'neighb" and neighb_insert :: "'a \<Rightarrow> 'neighb \<Rightarrow> 'neighb" and
-     neighb_delete :: "'a \<Rightarrow> 'neighb \<Rightarrow> 'neighb" and neighb_isin :: "'neighb \<Rightarrow> 'a \<Rightarrow> bool" and
-     neighb_set :: "'neighb \<Rightarrow> 'a set" and neighb_inv :: "'neighb \<Rightarrow> bool" and neighb_sel::"'neighb \<Rightarrow> 'a" +
+     neighb_empty :: "'neighb"  ("\<emptyset>\<^sub>N") and neighb_delete :: "'a \<Rightarrow> 'neighb \<Rightarrow> 'neighb" and
+     neighb_insert and neighb_inv and isin +
 
-fixes adj_foreach :: "('a \<Rightarrow> 'neighb \<Rightarrow> 'neighb) \<Rightarrow> 'adj \<Rightarrow> 'neighb \<Rightarrow> 'neighb"
-assumes 
-   adj_foreach[simp]: "adj_inv adj_map \<Longrightarrow> (\<exists>xs. adj_foreach f adj_map a0 =  fold f xs a0 \<and> set xs = dom (adj_lookup adj_map))"
+fixes adj_foreach :: "('a \<Rightarrow> 'a set \<Rightarrow> 'a set) \<Rightarrow> 'adj \<Rightarrow> 'a set \<Rightarrow> 'a set"
+assumes
+   adj_foreach[simp]:
+    "adj_inv adj_map \<Longrightarrow> (\<exists>xs. adj_foreach f adj_map a0 =  fold f xs a0 \<and> set xs = dom (lookup adj_map))"
    \<comment> \<open>Every folding function that is needed for the domain of the map or the elements of the set
        can be added explicitly like this. There is no need to fix the function, but we need to fix
        its type.\<close>
-
-locale Pair_Graph_Specs = 
-  Adj_Map_Specs adj_empty adj_update adj_delete adj_lookup adj_inv neighb_empty neighb_insert neighb_delete neighb_isin neighb_set neighb_inv neighb_sel adj_foreach
-
- for adj_empty :: "'adj" and adj_update :: "'a \<Rightarrow> 'neighb \<Rightarrow> 'adj \<Rightarrow> 'adj" and
-     adj_delete :: "'a \<Rightarrow> 'adj \<Rightarrow> 'adj" and adj_lookup :: "'adj \<Rightarrow> 'a \<Rightarrow> 'neighb option" and
-     adj_inv :: "'adj \<Rightarrow> bool"  and
-
-     neighb_empty :: "'neighb" and neighb_insert :: "'a \<Rightarrow> 'neighb \<Rightarrow> 'neighb" and
-     neighb_delete :: "'a \<Rightarrow> 'neighb \<Rightarrow> 'neighb" and neighb_isin :: "'neighb \<Rightarrow> 'a \<Rightarrow> bool" and
-     neighb_set :: "'neighb \<Rightarrow> 'a set" and neighb_inv :: "'neighb \<Rightarrow> bool" and neighb_sel::"'neighb \<Rightarrow> 'a"
-     and neighb_foreach :: "('a \<Rightarrow> 'b \<Rightarrow> 'b) \<Rightarrow> 'neighb \<Rightarrow> 'b \<Rightarrow> 'b" and
-
-     adj_foreach :: "('a \<Rightarrow> 'neighb \<Rightarrow> 'neighb) \<Rightarrow> 'adj \<Rightarrow> 'neighb \<Rightarrow> 'neighb" +
-
-fixes digraph::"'adj" 
-assumes digraph_invar[simp]:
-   "adj_inv digraph" and
-   \<comment> \<open>This is because in the abstract graph model we have no disconnected vertices.\<close>
-   neighbourhood_invars[intro]:
-   "(adj_lookup digraph v = Some neighb) \<Longrightarrow> set (neighb_inorder neighb) \<noteq> {}"
-   "adj_lookup digraph v = Some neighb \<Longrightarrow> neighb_invar neighb"
+  \<comment> \<open>Why do we need ann efficient neghbourhood test?\<close>
 
 begin
+
+abbreviation isin' (infixl "\<in>\<^sub>G" 50) where "isin' G v \<equiv> isin v G" 
+abbreviation not_isin' (infixl "\<notin>\<^sub>G" 50) where "not_isin' G v \<equiv> \<not> isin' G v"
+
+
+end
+
+locale Pair_Graph_Specs = 
+  Adj_Map_Specs where update = update
+for update :: "'a \<Rightarrow> 'neighb \<Rightarrow> 'adj \<Rightarrow> 'adj"  +
+
+fixes digraph::"'adj" 
+assumes digraph_invar:
+   "adj_inv digraph" and
+   \<comment> \<open>This is because in the abstract graph model we have no disconnected vertices.\<close>
+   neighbourhood_invars:
+   "(lookup digraph v = Some neighb)"
+   "lookup digraph v = Some neighb \<Longrightarrow> neighb_inv neighb"
+
+begin
+
 
 declare adj.map_empty[simp] adj.map_update[simp] adj.map_delete[simp] adj.invar_empty[simp]
         adj.invar_update[simp] adj.invar_delete[simp]
@@ -67,126 +96,40 @@ declare adj.map_empty[simp] adj.map_update[simp] adj.map_delete[simp] adj.invar_
 declare neighb.set_empty[simp] neighb.set_isin[simp] neighb.set_insert[simp] neighb.set_delete[simp]
         neighb.invar_empty[simp] neighb.invar_insert[simp] neighb.invar_delete[simp] neighb.choose[simp]
 
-definition neighbourhood::"'a \<Rightarrow> 'neighb option" where "neighbourhood v \<equiv> adj_lookup digraph v"
+definition neighbourhood::"'a \<Rightarrow> 'neighb" where "neighbourhood v \<equiv> the (lookup digraph v)"
 
-definition neighbourhood_abs::"'a \<Rightarrow> 'a set" where
- "neighbourhood_abs u \<equiv> case neighbourhood u of Some neighb \<Rightarrow> (neighb_set neighb) | _ \<Rightarrow> {}"
+notation "neighbourhood" ("\<N>\<^sub>G _" 100)
 
-definition vertices::"'neighb" where
-  "vertices \<equiv> adj_foreach (\<lambda>v. neighb_insert v) digraph neighb_empty"
+lemma neighbourhood_invars'[simp]:
+   "neighb_inv (\<N>\<^sub>G v)"
+  by (auto simp add: neighbourhood_def neighbourhood_invars)
 
-definition vertices_abs::"'a set" where
-  "vertices_abs \<equiv> neighb_set vertices"
-
-definition are_connected::"'a \<Rightarrow> 'a \<Rightarrow> bool" where
-  "are_connected u v = (case (neighbourhood u) of Some neighb \<Rightarrow> neighb_isin neighb v | _ \<Rightarrow> False)"
-
-definition "digraph_abs \<equiv> {(u,v). v \<in> (neighbourhood_abs u) \<and> u \<in> vertices_abs}"
+definition "digraph_abs \<equiv> {(u,v). v \<in>\<^sub>G (\<N>\<^sub>G u)}"
 
 subsection \<open>Abstraction lemmas\<close>
 
-text \<open>The idea here is use these lemmas in automation to transform all proof obligations to 
-      abstract data structures.\<close>
+text \<open>These are lemmas for automation. Their purpose is to remove any mention of the neighbourhood
+      concept implemented using the locale constructs and replace it with abstract terms
+      on pair graphs.\<close>
 
-lemma are_connected_abs[simp]: 
-  "are_connected u v \<longleftrightarrow> (u,v) \<in> digraph_abs"
-  by(auto simp: are_connected_def digraph_abs_def neighbourhood_abs_def neighbourhood_def
-                   vertices_abs_def option.discI
-             split: option.split)
+lemma are_connected_abs: 
+  "v \<in> t_set (\<N>\<^sub>G u) \<longleftrightarrow> (u,v) \<in> digraph_abs"
+  by(auto simp: digraph_abs_def neighbourhood_def option.discI neighbourhood_invars
+          split: option.split)
 
-lemma neighbourhood_abs_fold: 
-  "set vs = dom (adj_lookup digraph) \<Longrightarrow>
-         neighb_set (fold (\<lambda>v. neighb_insert v) vs neighb_empty) = dVs digraph_abs"
-  by (induction vs arbitrary: )
-     (auto simp: dVs_def digraph_abs_def neighbourhood_abs_def neighbourhood_def vertices_abs_def
-                 vertices_def
-           split: option.splits)
+lemma are_connected_absD[dest!]: 
+  "v \<in> t_set (\<N>\<^sub>G u) \<Longrightarrow> (u,v) \<in> digraph_abs"
+  by (auto simp: are_connected_abs)
 
-lemma neighbourhood_abs: "neighb_set vertices = dVs digraph_abs"
-  apply(simp add: vertices_def)
-  by (metis adj_foreach digraph_invar neighbourhood_abs_fold)
+lemma are_connected_absI[intro!]: 
+  "(u,v) \<in> digraph_abs \<Longrightarrow> v \<in> t_set (\<N>\<^sub>G u)"
+  by (auto simp: are_connected_abs)
 
 
-lemma neighbourhood_inv_fold: 
-  "set vs = dom (adj_lookup digraph) \<Longrightarrow>
-         neighb_inv (fold (\<lambda>v. neighb_insert v) vs neighb_empty)"
-  by (induction vs arbitrary: ) auto
-
-lemma inv_vertices: "neighb_inv (vertices)"
-  apply(simp add: vertices_def)        
-  by (metis adj_foreach digraph_invar neighbourhood_inv_fold)
-
-lemma neighbourhood_abs_in: "neighb_isin vertices v \<longleftrightarrow> v \<in> dVs digraph_abs"
-  by(auto simp add: neighbourhood_abs inv_vertices)
+lemma neighbourhood_absD[dest!]:
+  "t_set (\<N>\<^sub>G x) \<noteq> {} \<Longrightarrow> x \<in> dVs digraph_abs"
+  by (auto simp: digraph_abs_def dVs_def dest!: neighb.emptyD)
 
 end  
-
-locale Pair_Graph_Specs_by_Ordered = 
- adj: Map_by_Ordered adj_empty adj_update adj_delete adj_lookup adj_inorder adj_inv +
-
- neighb: Set_by_Ordered neighb_empty neighb_insert neighb_delete neighb_isin neighb_inorder neighb_inv 
-
- for adj_empty :: "'adj" and adj_update :: "'a::linorder \<Rightarrow> 'neighb \<Rightarrow> 'adj \<Rightarrow> 'adj" and
-     adj_delete :: "'a \<Rightarrow> 'adj \<Rightarrow> 'adj" and adj_lookup :: "'adj \<Rightarrow> 'a \<Rightarrow> 'neighb option" and
-     adj_inorder :: "'adj \<Rightarrow> ('a * 'neighb) list" and adj_inv :: "'adj \<Rightarrow> bool" and
-
-     neighb_empty :: "'neighb" and neighb_insert :: "'a::linorder \<Rightarrow> 'neighb \<Rightarrow> 'neighb" and
-     neighb_delete :: "'a \<Rightarrow> 'neighb \<Rightarrow> 'neighb" and neighb_isin :: "'neighb \<Rightarrow> 'a \<Rightarrow> bool" and
-     neighb_inorder :: "'neighb \<Rightarrow> 'a list" and neighb_inv :: "'neighb \<Rightarrow> bool" +
-
-fixes digraph::"'adj"
-
-assumes digraph_invar[simp]:
-   "adj_inv digraph" and
-   \<comment> \<open>This is because in the abstract graph model we have no disconnected vertices.\<close>
-   neighbourhood_invars[intro]:
-   "(adj_lookup digraph v = Some neighb) \<Longrightarrow> set (neighb_inorder neighb) \<noteq> {}"
-   "adj_lookup digraph v = Some neighb \<Longrightarrow> neighb_invar neighb"
-
-begin
-
-declare adj.inorder_empty[simp] adj.inorder_lookup[simp] adj.inorder_update[simp]
-        adj.inorder_delete[simp] adj.inorder_inv_empty[simp] adj.inorder_inv_update[simp]
-        adj.inorder_inv_delete[simp]
-
-declare neighb.inorder_empty[simp] neighb.isin[simp] neighb.inorder_insert[simp]
-        neighb.inorder_delete[simp] neighb.inorder_inv_empty[simp] neighb.inorder_inv_insert[simp]
-        neighb.inorder_inv_delete[simp]
-
-
-definition neighbourhood::"'a \<Rightarrow> 'neighb option" where "neighbourhood v \<equiv> adj_lookup digraph v"
-
-definition neighbourhood_abs::"'a \<Rightarrow> 'a set" where
- "neighbourhood_abs u \<equiv> case neighbourhood u of Some neighb \<Rightarrow> set (neighb_inorder neighb) | _ \<Rightarrow> {}"
-
-definition vertices::"'neighb" where
-  "vertices \<equiv> fold (\<lambda>(v,neighb). neighb_insert v) (adj_inorder digraph) neighb_empty"
-
-definition vertices_abs::"'a set" where
-  "vertices_abs \<equiv> set (neighb_inorder vertices)"
-
-definition are_connected::"'a \<Rightarrow> 'a \<Rightarrow> bool" where
-  "are_connected u v = (case (neighbourhood u) of Some neighb \<Rightarrow> neighb_isin neighb v | _ \<Rightarrow> False)"
-
-definition "digraph_abs \<equiv> {(u,v). v \<in> (neighbourhood_abs u) \<and> u \<in> vertices_abs}"
-
-subsection \<open>Abstraction lemmas\<close>
-
-text \<open>The idea here is use these lemmas in automation to transform all proof obligations to 
-      abstract data structures.\<close>
-
-lemma are_connected_abs[simp]: 
-  "are_connected u v \<longleftrightarrow> (u,v) \<in> digraph_abs"
-  by(auto simp: are_connected_def digraph_abs_def neighbourhood_abs_def neighbourhood_def
-                   vertices_abs_def option.discI
-             split: option.split)
-
-lemma "vertices_abs = dVs digraph_abs" 
-  sorry
-
-
-end  
-
-
 
 end
